finished soundness proof for get_respectful.

Charge!/src/Charge/Tactics/PullQuant/PullQuantRtac.v
@@ -23,6 +23,7 @@ Section parametric.
   Context {Typ0_Prop : Typ0 _ Prop}.
   Context {Typ0Ok_Fun : Typ0Ok Typ0_Prop}.
   Variable RelDec_typ : RelDec (@eq typ).
+  Variable RelDec_Correct_typ : RelDec_Correct RelDec_typ.
   Variable lops : logic_ops.
   Variable lopsOk : logic_opsOk lops.
   Context {ViewFunc_ilogic : FuncView func (ilfunc typ)}.
@@ -186,38 +187,37 @@ Section parametric.
     { simpl. intros; congruence. }
   Qed.
 
+  Definition if_entails (t : typ) Y (X : expr typ func) : mrw (list (R typ (expr typ func))) :=
+    run_default (inj (ptrn_view _ (pmap (fun t' => if t ?[ eq ] t' then rw_ret Y else rw_fail)
+                                        (fptrnEntails get)))) (rw_fail) X.
+
   (** This function defines what terms respect what relations **)
   Definition get_respectful
              (e : expr typ func) (r : R typ (expr typ func))
-  : list (R typ (expr typ func)) :=
-    let if_entails Y X :=
-        run_default (inj (ptrn_view _ (pmap (fun _ =>
-                                               Y) (fptrnEntails get)))) nil X
-    in
+  : mrw (list (R typ (expr typ func))) :=
     run_default (Ptrns.inj (ptrn_view _
          (pors
-           (pmap (fun l_t => let '(l,t) := l_t in
+           (pmap (fun t_l => let '(t,l) := t_l in
                              match r with
                              | Rinj X
                              | Rflip (Rinj X) =>
-                               if_entails (Rrespects (Rpointwise t r) r :: nil)
-                                          X
-                             | _ => nil
+                               if_entails l (Rpointwise t r :: nil) X
+                             | _ => rw_fail
                              end) (fptrnExists get) ::
             pmap (fun l => match r with
                             | Rinj X
                             | Rflip (Rinj X) =>
-                              if_entails (Rrespects r (Rrespects r r) :: nil) X
-                            | _ => nil
+                              if_entails l (r :: r :: nil) X
+                            | _ => rw_fail
                             end) (por (fptrnAnd get) (fptrnOr get)) ::
             pmap (fun l => match r with
                             | Rinj X
                             | Rflip (Rinj X) =>
-                              if_entails (Rrespects (Rflip' r) (Rrespects r r) :: nil) X
-                            | _ => nil
+                              if_entails l (Rflip' r :: r :: nil) X
+                            | _ => rw_fail
                             end) (fptrnImpl get) ::
             nil))))
-       nil
+       (rw_fail)
        e.
 
   (* This was necessary for post-processing the substitution *)
@@ -319,7 +319,509 @@ Section parametric.
                   bottom_up (is_reflR is_refl)
                             (is_transR is_trans)
                             (the_prewrites the_lemmas)
-                            (fun e r => rw_ret (get_respectful e r)) e r).
+                            (get_respectful) e r).
+
+  Ltac Rty_inv :=
+    let rec find A B more none :=
+        match A with
+        | B => none tt
+        | typ1 ?A' =>
+          match B with
+          | typ1 ?B' => find A' B' more none
+          | _ => let r := constr:(A = B) in more r
+          end
+        | typ2 ?A1' ?A2' =>
+          match B with
+          | typ2 ?B1' ?B2' =>
+            let m' x := find A2' B2' ltac:(fun y => let r := constr:(x /\ y) in more r) ltac:(fun _ => more x) in
+            let n' x := find A2' B2' more none in
+            find A1' B1' m' n'
+          | _ => let r := constr:(A = B) in more r
+          end
+        | _ => let r := constr:(A = B) in more r
+        end
+    in
+    let rec break_ands H P :=
+        match P with
+        | ?A /\ ?B =>
+          let H1 := fresh in
+          let H2 := fresh in
+          destruct H as [ H1 H2 ]; break_ands H1 A ; break_ands H2 B
+        | _ => idtac
+        end
+    in
+    let finish Hstart P :=
+        let H := fresh in
+        assert (H : P) by (inv_all; eauto) ;
+          break_ands H P ; repeat progress subst ;
+          try ( rewrite (UIP_refl Hstart) in * ) ; try clear Hstart
+    in
+    match goal with
+    | H : Rty ?A ?B |- _ =>
+      find A B ltac:(fun x => finish H x) ltac:(fun _ => fail)
+    | H : @eq (option typ) (Some ?A) (Some ?B) |- _ =>
+      find A B ltac:(fun x => finish H x) ltac:(fun _ => fail)
+    end.
+
+
+  Lemma if_entails_sound : forall t X r a b c d e f g h i,
+      @if_entails t X r a b c d e f g = Some (h,i) -> 
+      g = i /\ h = X /\ r = Inj (f_insert (ilf_entails t)).
+  Proof.
+    intros. revert H.
+    unfold if_entails.
+    eapply run_default_sound; eauto 100 with typeclass_instances.
+    { intros. ptrnE.
+      eapply Succeeds_ptrn_view in H2; eauto 100 with typeclass_instances.
+      destruct H2 as [ ? [ ? ? ] ].
+      subst. ptrnE.
+      consider (t ?[ eq ] x).
+      { intros. inversion H0; clear H0; subst.
+        split; auto. }
+      { inversion 2. } }
+    { inversion 1. }
+  Qed.
+
+  Lemma acc_fold_right
+    : forall t ts t',
+      TransitiveClosure.leftTrans (tyAcc (typ:=typ))
+                                  t (fold_right (typ2 (F:=Fun)) t (t'::ts)).
+  Proof.
+    induction ts.
+    { simpl; intros. constructor. eapply tyAcc_typ2R; eauto. }
+    { intros. specialize IHts.
+      specialize (IHts a).
+      simpl. eapply TransitiveClosure.leftTrans_rightTrans.
+      eapply TransitiveClosure.RTStep.
+      eapply TransitiveClosure.leftTrans_rightTrans. eassumption.
+      eapply tyAcc_typ2R; eauto. }
+  Qed.
+
+  Lemma Rty_fold_right
+    : forall y x ts,
+      Rty (fold_right (typ2 (F:=Fun)) x ts) (typ2 y x) ->
+      ts = y :: nil.
+  Proof.
+    intros. red in H.
+    destruct ts; simpl in *.
+    { eapply AppN.tyArr_circ_R in H; eauto. destruct H. }
+    eapply typ2_inj in H; eauto.
+    destruct H. destruct H.
+    destruct ts.
+    { reflexivity. }
+    { exfalso.
+      generalize (acc_fold_right x ts t0).
+      assert (well_founded (TransitiveClosure.leftTrans (tyAcc (typ:=typ)))).
+      { eapply Relation.wf_leftTrans.
+        eapply wf_tyAcc; eauto. }
+      intro. eapply Facts.wf_anti_sym in H.
+      rewrite H0 in H1.
+      eapply H. eassumption. }
+  Qed.
+
+  Lemma Rty_fold_right2
+    : forall y x z ts,
+      Rty (fold_right (typ2 (F:=Fun)) x ts) (typ2 y (typ2 z x)) ->
+      ts = y :: z :: nil.
+  Proof.
+    intros. red in H.
+    destruct ts.
+    { exfalso.
+      simpl in *.
+      assert (well_founded (TransitiveClosure.leftTrans (tyAcc (typ:=typ)))).
+      { eapply Relation.wf_leftTrans.
+        eapply wf_tyAcc; eauto. }
+      eapply Facts.wf_anti_sym in H0.
+      eapply H0. instantiate (1 := x).
+      rewrite H at 2.
+      eapply TransitiveClosure.leftTrans_rightTrans.
+      eapply TransitiveClosure.RTStep.
+      2: eapply tyAcc_typ2R; eauto.
+      constructor.
+      eapply tyAcc_typ2R; eauto. }
+    simpl in H.
+    apply typ2_inj in H; eauto. destruct H.
+    destruct H.
+    eapply Rty_fold_right in H0. subst. reflexivity.
+  Qed.
+
+  Lemma RbaseD_entails'
+    : forall t t' rD,
+      RbaseD (Inj (f_insert (ilf_entails t'))) t = Some rD ->
+      t = t' /\
+      exists L,
+        lops t = _Some L /\
+        rD = ILogic.lentails.
+  Proof.
+    unfold RbaseD, exprD; simpl.
+    intros. autorewrite with exprD_rw in H.
+    simpl in H.
+    rewrite <- (@fv_compat _ _ _ _ _ _ _ ViewFuncOk_ilogic) in H.
+    unfold symAs, typeof_sym in H. simpl in H.
+    rewrite castD_option in H.
+    destruct (lops t') eqn:heq; try solve [ inversion H ].
+    forwardy.
+    inv_all. subst.
+    Rty_inv. Rty_inv. split; auto.
+    eexists; split; eauto.
+    rewrite type_cast_refl in H by eauto.
+    inv_all.
+    simpl in H.
+    unfold entailsR. simpl. unfold id.
+    rewrite castDR. auto.
+  Qed.
+
+  Lemma RbaseD_entails
+    : forall t rD,
+      RbaseD (Inj (f_insert (ilf_entails t))) t = Some rD ->
+      exists L,
+        lops t = _Some L /\
+        rD = ILogic.lentails.
+  Proof.
+    unfold RbaseD, exprD; simpl.
+    intros. autorewrite with exprD_rw in H.
+    simpl in H.
+    rewrite <- (@fv_compat _ _ _ _ _ _ _ ViewFuncOk_ilogic) in H.
+    unfold symAs, typeof_sym in H. simpl in H.
+    rewrite castD_option in H.
+    destruct (lops t); try solve [ inversion H ].
+    eexists; split; eauto.
+    rewrite type_cast_refl in H by eauto.
+    inv_all.
+    simpl in H.
+    unfold entailsR in H.
+    rewrite castDR in H. auto.
+  Qed.
+
+  Lemma binary_inference
+  : let rs_log := @RSym_ilfunc typ _ _ _ _ lops in
+    forall (X : ilfunc typ) t x ts r rD x0,
+      (r = Rinj (Inj (f_insert (ilf_entails x))) \/
+       r = Rflip (Rinj (Inj (f_insert (ilf_entails x))))) ->
+      RD RbaseD r t = Some rD ->
+      symAs X (fold_right (typ2 (F:=Fun)) t ts) = Some x0 ->
+      typeof_sym X = Some (typ2 (F:=Fun) x (typ2 (F:=Fun) x x)) ->
+      t = x /\ ts = t :: t :: nil.
+  Proof.
+    unfold symAs, RbaseD, exprD; simpl.
+    destruct 1; simpl; subst; simpl; intros.
+    { generalize dependent (funcD lops X).
+      rewrite H1.
+      intros. forwardy.
+      clear H2 H0.
+      autorewrite with exprD_rw in H. simpl in H.
+      rewrite <- (@fv_compat _ _ _ _ _ _ _ ViewFuncOk_ilogic) in H.
+      unfold symAs, typeof_sym in H; simpl in H.
+      rewrite castD_option in H.
+      destruct (lops x); [ inversion H | ].
+      forwardy.
+      inv_all. subst.
+      Rty_inv. Rty_inv.
+      split; auto.
+      eapply Rty_fold_right2.
+      eauto. }
+    { generalize dependent (funcD lops X).
+      rewrite H1.
+      intros. forwardy.
+      clear H2 H0.
+      autorewrite with exprD_rw in H. simpl in H.
+      rewrite <- (@fv_compat _ _ _ _ _ _ _ ViewFuncOk_ilogic) in H.
+      unfold symAs, typeof_sym in H; simpl in H.
+      rewrite castD_option in H.
+      destruct (lops x); [ inversion H | ].
+      forwardy.
+      inv_all. subst.
+      Rty_inv. Rty_inv.
+      split; auto.
+      eapply Rty_fold_right2.
+      eauto. }
+  Qed.
+
+  (** It would be nice if we could prove this more quickly *)
+  Theorem get_respectful_sound
+  : respectful_spec RbaseD get_respectful.
+  Proof.
+    red. intros.
+    generalize dependent e. intro.
+    unfold get_respectful.
+    eapply run_default_sound.
+    { eauto 100 with typeclass_instances. }
+    { intros.
+      ptrnE.
+      eapply Succeeds_ptrn_view in H3; eauto 100 with typeclass_instances.
+      destruct H3 as [ ? [ ? ? ] ].
+      repeat (ptrnE; try match goal with
+                         | H : _ \/ _ |- _ => destruct H
+                         end).
+      { assert (exists X, (r = Rinj X \/ r = Rflip (Rinj X)) /\
+                   if_entails t0 (Rpointwise t r :: nil) X tvs' (getUVars ctx) (getVars ctx) (length (getUVars ctx))
+                              (length (getVars ctx)) cs = Some (rs, cs')).
+        { destruct r; eauto; try solve [ inversion H1 ].
+          destruct r; eauto; try solve [ inversion H1 ]. }
+        clear H1. destruct H. destruct H.
+        eapply if_entails_sound in H1.
+        destruct H1 as [ ? [ ? ? ] ]. subst.
+        split; auto. intros.
+        forward.
+        simpl.
+        autorewrite with exprD_rw in H2. simpl in H2.
+        forwardy. inv_all. subst.
+
+        assert (t1 = t0 /\ ts = typ2 t t0 :: nil).
+        { eapply ExprFacts.symAs_typeof_sym in H3.
+          simpl in H3.
+          destruct (lops t0) eqn:Heq; [ inversion H3 | ].
+          inv_all.
+          assert (t1 = t0).
+          { destruct H; subst.
+            simpl in H1.
+            eapply RbaseD_entails' in H1; tauto.
+            simpl in H1.
+            forwardy.
+            eapply RbaseD_entails' in H; tauto. }
+          subst. split; auto.
+          eapply Rty_fold_right. symmetry. eassumption. }
+        destruct H4; subst.
+        simpl.
+        repeat rewrite typ2_match_iota by eauto.
+        rewrite type_cast_refl by eauto.
+        rewrite H1.
+        autorewrite_with_eq_rw.
+        split; [ reflexivity | ].
+        intros.
+        eapply Pure_pctxD; eauto. intros.
+        unfold Morphisms.Proper.
+        autorewrite_with_eq_rw.
+
+        destruct H; subst.
+        { eapply RbaseD_entails in H1.
+          destruct H1 as [ ? [ ? ? ] ].
+          subst.
+          unfold symAs in H3.
+          simpl in H3.
+          rewrite H in H3.
+          rewrite type_cast_refl in H3 by eauto.
+          inv_all. subst.
+          simpl.
+          unfold respectful, existsR.
+          specialize (lopsOk t0). rewrite H in lopsOk.
+          clear - lopsOk.
+          unfold castR. simpl.
+          generalize (typ2_cast (typ2 t t0) t0).
+          generalize (typ2_cast t t0).
+          generalize (typD (typ2 t t0)).
+          generalize (typD (typ2 (typ2 t t0) t0)).
+          intros; subst. simpl in *.
+          eapply ILogic.lexists_lentails_m.
+          red. intros. eapply H. }
+        { simpl in H1. forwardy.
+          eapply RbaseD_entails in H.
+          destruct H as [ ? [ ? ? ] ].
+          subst.
+          unfold symAs in H3.
+          simpl in H3.
+          rewrite H in H3.
+          rewrite type_cast_refl in H3 by eauto.
+          inv_all. subst.
+          simpl.
+          unfold respectful, existsR.
+          specialize (lopsOk t0). rewrite H in lopsOk.
+          clear - lopsOk.
+          unfold castR. simpl.
+          generalize (typ2_cast (typ2 t t0) t0).
+          generalize (typ2_cast t t0).
+          generalize (typD (typ2 t t0)).
+          generalize (typD (typ2 (typ2 t t0) t0)).
+          intros; subst. simpl in *.
+          eapply ILogic.lexists_lentails_m.
+          red. intros. eapply H. } }
+      { (* AND *)
+        assert (exists X, (r = Rinj X \/ r = Rflip (Rinj X)) /\
+                   if_entails x (r :: r :: nil) X tvs' (getUVars ctx) (getVars ctx) (length (getUVars ctx))
+                              (length (getVars ctx)) cs = Some (rs, cs')).
+        { destruct r; eauto; try solve [ inversion H1 ].
+          destruct r; eauto; try solve [ inversion H1 ]. }
+        clear H1. destruct H. destruct H.
+        eapply if_entails_sound in H1.
+        destruct H1 as [ ? [ ? ? ] ]. subst.
+        split; auto. intros.
+        forward.
+        simpl.
+        autorewrite with exprD_rw in H2. simpl in H2.
+        forwardy. inv_all. subst.
+        generalize (@binary_inference (ilf_and x) _ _ _ _ _ _ H H1 H3).
+        unfold symAs, typeof_sym in H3; simpl in H3.
+        simpl.
+        destruct (lops x) eqn:Hlops; try solve [ inversion H3 ].
+        intro Hx; specialize (Hx eq_refl); destruct Hx; subst.
+        simpl.
+        rewrite type_cast_refl in * by eauto.
+        inv_all. subst.
+        repeat rewrite typ2_match_iota by eauto.
+        rewrite H1.
+        autorewrite_with_eq_rw.
+        split; [ reflexivity | ].
+        intros.
+        eapply Pure_pctxD; eauto. intros.
+        unfold Morphisms.Proper.
+        autorewrite_with_eq_rw.
+
+        destruct H; subst.
+        { eapply RbaseD_entails in H1.
+          destruct H1 as [ ? [ ? ? ] ].
+          rewrite Hlops in H. inversion H; clear H; subst.
+          specialize (lopsOk x).
+          rewrite Hlops in lopsOk.
+          clear - lopsOk.
+          unfold respectful, andR, castR. simpl.
+          generalize (typ2_cast x (typ2 x x)).
+          generalize (typ2_cast x x).
+          generalize (typD (typ2 x x)).
+          generalize (typD (typ2 x (typ2 x x))).
+          intros; subst; simpl.
+          intros. rewrite H. rewrite H0. reflexivity. }
+        { simpl in H1. forwardy.
+          eapply RbaseD_entails in H.
+          destruct H as [ ? [ ? ? ] ].
+          inv_all; subst.
+          specialize (lopsOk x).
+          rewrite Hlops in lopsOk.
+          rewrite Hlops in H. inversion H. subst.
+          clear - lopsOk.
+          unfold respectful, andR, castR. simpl.
+          generalize (typ2_cast x (typ2 x x)).
+          generalize (typ2_cast x x).
+          generalize (typD (typ2 x x)).
+          generalize (typD (typ2 x (typ2 x x))).
+          intros; subst; simpl.
+          intros. unfold flip in *.
+          rewrite H. rewrite H0. reflexivity. } }
+      { (* OR *)
+        assert (exists X, (r = Rinj X \/ r = Rflip (Rinj X)) /\
+                   if_entails x (r :: r :: nil) X tvs' (getUVars ctx) (getVars ctx) (length (getUVars ctx))
+                              (length (getVars ctx)) cs = Some (rs, cs')).
+        { destruct r; eauto; try solve [ inversion H1 ].
+          destruct r; eauto; try solve [ inversion H1 ]. }
+        clear H1. destruct H. destruct H.
+        eapply if_entails_sound in H1.
+        destruct H1 as [ ? [ ? ? ] ]. subst.
+        split; auto. intros.
+        forward.
+        simpl.
+        autorewrite with exprD_rw in H2. simpl in H2.
+        forwardy. inv_all. subst.
+        generalize (@binary_inference (ilf_or x) _ _ _ _ _ _ H H1 H3).
+        unfold symAs, typeof_sym in H3; simpl in H3.
+        simpl.
+        destruct (lops x) eqn:Hlops; try solve [ inversion H3 ].
+        intro Hx; specialize (Hx eq_refl); destruct Hx; subst.
+        simpl.
+        rewrite type_cast_refl in * by eauto.
+        inv_all. subst.
+        repeat rewrite typ2_match_iota by eauto.
+        rewrite H1.
+        autorewrite_with_eq_rw.
+        split; [ reflexivity | ].
+        intros.
+        eapply Pure_pctxD; eauto. intros.
+        unfold Morphisms.Proper.
+        autorewrite_with_eq_rw.
+
+        destruct H; subst.
+        { eapply RbaseD_entails in H1.
+          destruct H1 as [ ? [ ? ? ] ].
+          rewrite Hlops in H. inversion H; clear H; subst.
+          specialize (lopsOk x).
+          rewrite Hlops in lopsOk.
+          clear - lopsOk.
+          unfold respectful, orR, castR. simpl.
+          generalize (typ2_cast x (typ2 x x)).
+          generalize (typ2_cast x x).
+          generalize (typD (typ2 x x)).
+          generalize (typD (typ2 x (typ2 x x))).
+          intros; subst; simpl.
+          intros. rewrite H. rewrite H0. reflexivity. }
+        { simpl in H1. forwardy.
+          eapply RbaseD_entails in H.
+          destruct H as [ ? [ ? ? ] ].
+          inv_all; subst.
+          specialize (lopsOk x).
+          rewrite Hlops in lopsOk.
+          rewrite Hlops in H. inversion H. subst.
+          clear - lopsOk.
+          unfold respectful, orR, castR. simpl.
+          generalize (typ2_cast x (typ2 x x)).
+          generalize (typ2_cast x x).
+          generalize (typD (typ2 x x)).
+          generalize (typD (typ2 x (typ2 x x))).
+          intros; subst; simpl.
+          intros. unfold flip in *.
+          rewrite H. rewrite H0. reflexivity. } }
+      { (* Implication *)
+        assert (exists X, (r = Rinj X \/ r = Rflip (Rinj X)) /\
+                   if_entails x (Rflip' r :: r :: nil) X tvs' (getUVars ctx) (getVars ctx) (length (getUVars ctx))
+                              (length (getVars ctx)) cs = Some (rs, cs')).
+        { destruct r; eauto; try solve [ inversion H1 ].
+          destruct r; eauto; try solve [ inversion H1 ]. }
+        clear H1. destruct H. destruct H.
+        eapply if_entails_sound in H1.
+        destruct H1 as [ ? [ ? ? ] ]. subst.
+        split; auto. intros.
+        forward.
+        simpl.
+        autorewrite with exprD_rw in H2. simpl in H2.
+        forwardy. inv_all. subst.
+        generalize (@binary_inference (ilf_impl x) _ _ _ _ _ _ H H1 H3).
+        unfold symAs, typeof_sym in H3; simpl in H3.
+        simpl.
+        destruct (lops x) eqn:Hlops; try solve [ inversion H3 ].
+        intro Hx; specialize (Hx eq_refl); destruct Hx; subst.
+        simpl.
+        rewrite type_cast_refl in * by eauto.
+        inv_all. subst.
+        repeat rewrite typ2_match_iota by eauto.
+        rewrite RD_Rflip'_Rflip. simpl.
+        rewrite H1.
+        autorewrite_with_eq_rw.
+        split; [ reflexivity | ].
+        intros.
+        eapply Pure_pctxD; eauto. intros.
+        unfold Morphisms.Proper.
+        autorewrite_with_eq_rw.
+
+        destruct H; subst.
+        { eapply RbaseD_entails in H1.
+          destruct H1 as [ ? [ ? ? ] ].
+          rewrite Hlops in H. inversion H; clear H; subst.
+          specialize (lopsOk x).
+          rewrite Hlops in lopsOk.
+          clear - lopsOk.
+          unfold respectful, implR, castR. simpl.
+          generalize (typ2_cast x (typ2 x x)).
+          generalize (typ2_cast x x).
+          generalize (typD (typ2 x x)).
+          generalize (typD (typ2 x (typ2 x x))).
+          intros; subst; simpl.
+          unfold flip in *.
+          intros. rewrite <- H. rewrite H0. reflexivity. }
+        { simpl in H1. forwardy.
+          eapply RbaseD_entails in H.
+          destruct H as [ ? [ ? ? ] ].
+          inv_all; subst.
+          specialize (lopsOk x).
+          rewrite Hlops in lopsOk.
+          rewrite Hlops in H. inversion H. subst.
+          clear - lopsOk.
+          unfold respectful, implR, castR. simpl.
+          generalize (typ2_cast x (typ2 x x)).
+          generalize (typ2_cast x x).
+          generalize (typD (typ2 x x)).
+          generalize (typD (typ2 x (typ2 x x))).
+          intros; subst; simpl.
+          intros. unfold flip in *.
+          rewrite <- H. rewrite H0. reflexivity. } } }
+    { inversion 1. }
+  Qed.
 
   Definition quant_pull (l : typ) (e : expr typ func)
   : mrw (Progressing (expr typ func)) :=
